src/Util/ZUtil/Definitions.v
@@ -1,0 +1,7 @@
+Require Import Coq.ZArith.ZArith.
+Require Import Crypto.Util.ZUtil.Notations.
+Local Open Scope Z_scope.
+
+Module Z.
+  Definition pow2_mod n i := (n &' (Z.ones i)).
+End Z.
