src/Util/ZUtil/Notations.v
@@ -1,0 +1,6 @@
+Require Import Coq.ZArith.BinInt.
+Require Import Crypto.Util.Notations.
+
+Infix ">>" := Z.shiftr : Z_scope.
+Infix "<<" := Z.shiftl : Z_scope.
+Infix "&'" := Z.land : Z_scope.
